Refactor universality, adding many files

src/CoreData/CapCup.v
@@ -22,3 +22,13 @@ Definition n_cup n := (n_swap (n) ↕ n_wire n) ⟷ (n_cup_unswapped n).
 
 Definition n_cap n := (n_cup n) ⊤.
 
+
+Lemma n_stacked_pf_1 {n} : (n + n = n * 2)%nat. Proof. lia. Qed.
+
+Lemma n_stacked_pf_2 {n} : (0 = n * 0)%nat. Proof. lia. Qed.
+
+Definition n_stacked_caps n : ZX (n + n) 0 :=
+  cast _ _ n_stacked_pf_1 n_stacked_pf_2 (n ⇑ ⊃).
+
+  Definition n_stacked_cups n : ZX 0 (n + n) :=
+  cast _ _ n_stacked_pf_2 n_stacked_pf_1 (n ⇑ ⊂).
