src/CoreData/Controlizer.v
@@ -1,0 +1,189 @@
+Require Import ZXCore Proportional CapCup Stacks ZXperm States Gadgets ZXperm.
+Import Setoid.
+
+
+Definition is_controlled_scalar c (zx : ZX 1 0) :=
+  state_0 ⟷ zx ∝= ⦰ /\
+  state_1 ⟷ zx ∝= c .* ⦰.
+
+Add Parametric Morphism c : (@is_controlled_scalar c) with signature
+  proportional_by_1 ==> iff as is_controlled_scalar_mor.
+Proof.
+  unfold is_controlled_scalar.
+  now intros ? ? ->.
+Qed.
+
+Definition is_controlled_state {n} (czx : ZX 1 n) :=
+  state_0 ⟷ czx ∝= uniform_state n.
+
+Add Parametric Morphism {n} : (@is_controlled_state n) with signature
+  proportional_by_1 ==> iff as is_controlled_state_mor.
+Proof.
+  unfold is_controlled_state.
+  now intros ? ? ->.
+Qed.
+
+Definition is_controlized {n m} (zx : ZX n m) (czx : ZX 1 (n + m)) :=
+  is_controlled_state czx /\
+  zx ∝= (/√2)^ (n + m) .* 
+    state_to_proc (state_1 ⟷ czx).
+
+Add Parametric Morphism {n m} : (@is_controlized n m) with signature
+  proportional_by_1 ==> proportional_by_1 ==> iff as is_controlized_mor.
+Proof.
+  unfold is_controlized.
+  intros ? ? Hrw ? ? ->.
+  now rewrite Hrw.
+Qed.
+
+
+(* TODO: We can remove this, I believe *)
+Definition controlled_half : ZX 1 0 :=
+  zx_half ↕ (▷ ⟷ Z 1 0 0).
+
+
+
+Definition box_controlizer : ZX 1 (1 + 1) :=
+  (Z 1 2 0 ⟷ ((X 1 2 PI ⟷ (Z 1 0 (-(PI/4)) ↕ Z 1 0 (PI/4)) ⟷ 
+    Z 0 0 0) ↕
+    (X 1 2 PI ⟷ ((◁ ⟷ Z 1 2 0 ⟷ (— ↕ ◁)) ↕ —) ⟷ 
+    (— ↕ (Z 2 1 0 ⟷ □))))).
+
+
+Definition cupcap_controlizer : ZX 1 2 := 
+  Z 1 2 0 ⟷ ((◁ ⟷ Z 1 0 0 ⟷ X 0 1 0 ⟷ Z 1 0 0) ↕ 
+    (▷ ⟷ X 1 2 PI)).
+
+Definition swap_controlizer : ZX 1 (2 + 2) :=
+  (Z 1 3 0 ⟷ (Z 0 0 0 ↕ (◁ ⟷ Z 1 0 0) ↕ (◁ ⟷ Z 1 0 0) ↕ 
+    (X 1 1 PI ⟷ Z 1 2 0 ⟷ ((◁ ⟷ X 1 2 0) ↕ (◁ ⟷ X 1 2 0))
+    ⟷ (— ↕ (⨉ ↕ — ⟷ (— ↕ ⨉)))) )).
+
+
+Definition X_1_0_controlizer β : ZX 1 (1 + 0) := 
+  (Z 1 2 0 ⟷ ((◁ ⟷ Z 1 0 0) ↕ (X 1 1 PI ⟷ ◁ ⟷ X 1 1 β))).
+
+Definition X_1_2_controlizer : ZX 1 (1 + 2) :=
+  (Z 1 2 0 ⟷ ((◁ ⟷ Z 1 0 0 ⟷ Z 0 0 0) ↕ (▷ ⟷ X 1 3 PI))).
+
+Lemma comp_conlzr_prf1 {n m k} : (n + m + (m + k))%nat = (n + (m + m) + k)%nat.
+Proof. lia. Qed.
+
+Lemma comp_conlzr_prf2 {n k} : (n + k)%nat = (n + 0 + k)%nat.
+Proof. lia. Qed.
+
+
+
+Definition compose_controlizer {n m k} (czx0 : ZX 1 (n + m)) 
+  (czx1 : ZX 1 (m + k)) : 
+  ZX 1 (n + k) :=
+  (/2) ^ m .*
+  Z 1 2 0 ⟷ (czx0 ↕ czx1) ⟷
+  cast _ _ comp_conlzr_prf1 comp_conlzr_prf2
+    (n_wire n ↕ n_cup m ↕ n_wire k).
+
+
+Definition stack_controlizer {n m k l} (czx0 : ZX 1 (n + m)) 
+  (czx1 : ZX 1 (k + l)) : 
+  ZX 1 ((n + k) + (m + l)) :=
+  Z 1 2 0 ⟷ (czx0 ↕ czx1) ⟷
+  zx_invassoc (n + m) k l ⟷
+  ((zx_assoc n m k 
+    ⟷ (n_wire n ↕ zx_comm m k)
+    ⟷ zx_invassoc n k m) ↕ n_wire l) ⟷
+  zx_assoc (n + k) m l.
+
+
+Definition wire_controlizer : ZX 1 (1 + 1) :=
+  compose_controlizer box_controlizer box_controlizer.
+
+
+Definition half_controlizer : ZX 1 (0 + 0) :=
+  (zx_invsqrt2 ↕ zx_invsqrt2) ↕ (▷ ⟷ Z 1 0 0).
+
+Definition two_controlizer : ZX 1 (0 + 0) :=
+  ◁ ⟷ Z 1 0 0.
+
+Definition empty_controlizer : ZX 1 0 := 
+  stack_controlizer half_controlizer two_controlizer.
+
+
+Fixpoint n_stack_controlizer {n m} k (czx : ZX 1 (n + m)) : ZX 1 (k * n + k * m) :=
+  match k with
+  | 0 => empty_controlizer
+  | S k' => stack_controlizer czx (n_stack_controlizer k' czx)
+  end.
+
+Fixpoint n_stack1_controlizer k (czx : ZX 1 (1 + 1)) : ZX 1 (k + k) :=
+  match k with
+  | 0 => empty_controlizer
+  | S k' => stack_controlizer czx (n_stack1_controlizer k' czx)
+  end.
+
+Definition n_wire_controlizer n : ZX 1 (n + n) :=
+  n_stack1_controlizer n wire_controlizer.
+
+
+Definition X_2_1_controlizer : ZX 1 (2 + 1) := X_1_2_controlizer.
+
+Definition X_0_1_controlizer β : ZX 1 (0 + 1) := X_1_0_controlizer β.
+
+Fixpoint X_S_0_controlizer n β : ZX 1 (S n + 0) :=
+  match n with 
+  | 0 => X_1_0_controlizer β
+  | S n' => compose_controlizer
+    (stack_controlizer X_2_1_controlizer (n_wire_controlizer n'))
+    (X_S_0_controlizer n' β)
+  end.
+
+Fixpoint X_0_S_controlizer n β : ZX 1 (0 + S n) :=
+  match n with 
+  | 0 => X_0_1_controlizer β
+  | S n' => compose_controlizer
+    (X_0_S_controlizer n' β)
+    (stack_controlizer X_1_2_controlizer (n_wire_controlizer n'))
+  end.
+
+Definition X_0_n_controlizer n β : ZX 1 n :=
+  match n with 
+  | 0 => 
+    compose_controlizer (X_0_1_controlizer β) 
+      (X_1_0_controlizer 0)
+  | S n' => X_0_S_controlizer n' β
+  end.
+
+Definition X_controlizer n m β : ZX 1 (n + m) :=
+  X_0_n_controlizer (n + m) β.
+
+Definition Z_controlizer n m β : ZX 1 (n + m) :=
+  compose_controlizer (compose_controlizer
+    (n_stack1_controlizer n box_controlizer)
+    (X_controlizer n m β))
+    (n_stack1_controlizer m box_controlizer).
+
+Fixpoint controlizer {n m} (zx : ZX n m) : ZX 1 (n + m) :=
+  match zx with
+  | ⦰ => empty_controlizer
+  | — => wire_controlizer
+  | □ => box_controlizer
+  | ⊂ => cupcap_controlizer
+  | ⊃ => cupcap_controlizer
+  | ⨉ => swap_controlizer
+  | X n m α => X_controlizer n m α
+  | Z n m α => Z_controlizer n m α
+  | zx0 ↕ zx1 => stack_controlizer (controlizer zx0) (controlizer zx1)
+  | zx0 ⟷ zx1 => compose_controlizer (controlizer zx0) (controlizer zx1)
+  end.
+
+
+
+Lemma nn_n2 {n:nat} : (n + n = n * 2)%nat. Proof. lia. Qed.
+Definition sum_controlizer {n} (c0 c1 : ZX 1 n) : ZX 1 n :=
+  (X 0 1 0 ⟷ Z 1 0 0) ↕
+  (
+    Z 1 2 0 ⟷ (X 1 2 0 ↕ ◁) ⟷ (— ↕ Z 2 1 0) ⟷
+    (c0 ↕ c1)
+  ) ⟷
+  zx_of_perm_cast (n + n) (n * 2) (kron_comm_perm 2 n) nn_n2 ⟷
+  n ⇑ Z 2 1 0 ⟷
+  cast _ _ (Nat.mul_1_r n) eq_refl (n_wire n).
