src/CoreData/Gadgets.v
@@ -1,0 +1,155 @@
+Require Import ZXCore Proportional.
+
+From QuantumLib Require Complex Matrix RealAux Polar.
+
+Import Setoid.
+
+(* There are several functions we don't need or want exposed as
+  part of the main module, as they are just facts about C. If 
+  they were less ZX-specific, they could go in QuantumLib. *)
+Module ScalarC.
+
+Import Polar Modulus.
+
+Definition prop_lb (z : C) : nat := 
+  (BinInt.Z.to_nat (Int_part (ln (Cmod z / 2) / ln (√2))%R%C) + 1)%nat.
+
+(* Decomposition assuming |z| <= 2 *)
+Definition small_decomp (z : C) : R * R :=
+  let a := acos ((Cmod z)^2 / 2 - 1) in
+  (a, get_arg (z / (1 + Cexp a))).
+
+Definition prop_decomp (z : C) : nat * (R * R) :=
+  (prop_lb z, small_decomp (z / (√2 ^ prop_lb z))).
+
+End ScalarC.
+
+(* Some common values as gadgets *)
+
+Definition zx_sqrt2 : ZX 0 0 :=
+  Z 0 1 0 ⟷ X 1 0 PI.
+Lemma zx_sqrt2_defn : zx_sqrt2 =
+  Z 0 1 0 ⟷ X 1 0 PI.
+Proof. reflexivity. Qed.
+(* We don't ever want reduction to unfold zx_sqrt2 *)
+#[global]
+Opaque zx_sqrt2.
+
+Definition zx_invsqrt2 : ZX 0 0 :=
+  X 0 3 0 ⟷ Z 3 0 0.
+Lemma zx_invsqrt2_defn : zx_invsqrt2 =
+  X 0 3 0 ⟷ Z 3 0 0.
+Proof. reflexivity. Qed.
+(* We don't ever want reduction to unfold zx_invsqrt2 *)
+#[global]
+Opaque zx_invsqrt2.
+
+Definition zx_half : ZX 0 0 := zx_invsqrt2 ↕ zx_invsqrt2.
+Lemma zx_half_defn : zx_half = zx_invsqrt2 ↕ zx_invsqrt2.
+Proof. reflexivity. Qed.
+(* We don't ever want reduction to unfold zx_half *)
+#[global]
+Opaque zx_half.
+
+
+Definition zx_two : ZX 0 0 := Z 0 0 0.
+Lemma zx_two_defn : zx_two = Z 0 0 0.
+Proof. reflexivity. Qed.
+(* We don't ever want reduction to unfold zx_two *)
+#[global]
+Opaque zx_two.
+
+
+Definition zx_cexp (r : R) : ZX 0 0 :=
+  X 0 1 r ⟷ Z 1 0 PI ⟷ zx_invsqrt2.
+Lemma zx_cexp_defn (r : R) : zx_cexp r =
+  X 0 1 r ⟷ Z 1 0 PI ⟷ zx_invsqrt2.
+Proof. reflexivity. Qed.
+(* We don't ever want reduction to unfold zx_cexp *)
+#[global]
+Opaque zx_cexp.
+
+(* Gadget representing √2 ^ n as a diagram *)
+Fixpoint zx_nsqrt2 (n : nat) : ZX 0 0 :=
+  match n with 
+  | 0 => Empty
+  | S n' => zx_sqrt2 ⟷ zx_nsqrt2 n'
+  end.
+
+Import ScalarC.
+
+(* Gadget representing the scalar z as a ZX-diagram *)
+Definition zx_of_const (z : C) : ZX 0 0 :=
+  zx_nsqrt2 (fst (prop_decomp z)) ⟷
+  Z 0 0 (fst (snd (prop_decomp z))) ⟷
+  zx_cexp (snd (snd (prop_decomp z))).
+
+Lemma zx_of_const_defn (z : C) : zx_of_const z = 
+  zx_nsqrt2 (fst (prop_decomp z)) ⟷
+  Z 0 0 (fst (snd (prop_decomp z))) ⟷
+  zx_cexp (snd (snd (prop_decomp z))).
+Proof. reflexivity. Qed.
+(* We don't ever want reduction to unfold zx_of_const *)
+#[global]
+Opaque zx_of_const.
+
+
+Definition const_of_zx (zx : ZX 0 0) : C :=
+  ⟦ zx ⟧ O O.
+
+Add Parametric Morphism : const_of_zx 
+  with signature proportional_by_1 ==> eq as const_of_zx_mor.
+Proof.
+  intros zx zx' Hzx.
+  unfold const_of_zx.
+  now rewrite Hzx.
+Qed.
+
+Definition zx_scale {n m} (c : C) (zx : ZX n m) : ZX n m :=
+  zx_of_const c ↕ zx.
+
+Notation "c '.*' zx" := (zx_scale c zx) 
+  (at level 40, left associativity) : ZX_scope.
+
+Lemma zx_scale_defn {n m} c (zx : ZX n m) : c .* zx = zx_of_const c ↕ zx.
+Proof. reflexivity. Qed.
+
+Lemma zx_scale_fun_defn : @zx_scale = fun n m c zx => zx_of_const c ↕ zx.
+Proof. reflexivity. Qed.
+
+(* We really don't want zx_scale to reduce, as that'll be messy
+  (especially with dimensions!) *)
+#[global] Opaque zx_scale.
+
+Add Parametric Morphism {n m} c : (@zx_scale n m c) with signature 
+  proportional_by_1 ==> proportional_by_1 as zx_scale_prop_by_1_mor.
+Proof.
+  rewrite zx_scale_fun_defn.
+  intros zx0 zx1 ->.
+  reflexivity.
+Qed.
+
+Add Parametric Morphism {n m} c : (@zx_scale n m c) with signature 
+  proportional ==> proportional as zx_scale_mor.
+Proof.
+  rewrite zx_scale_fun_defn.
+  intros zx0 zx1 ->.
+  reflexivity.
+Qed.
+
+
+
+
+(* NB: Can be made effective using [Z 0 0 PI] for [0] *)
+Definition zx_zero {n m} : ZX n m :=
+  C0 .* Z n m 0.
+
+Lemma zx_zero_defn n m : zx_zero = C0 .* Z n m 0.
+Proof.
+  reflexivity.
+Qed.
+
+(* Don't unfold zx_zero *)
+Global Opaque zx_zero.
+
+Notation "0" := zx_zero : ZX_scope.
