src/CoreData/States.v
@@ -1,0 +1,90 @@
+Require Export ZXCore Proportional.
+Require Import CapCup Gadgets.
+
+
+(* The Choi-Jamiolchosky isomorphism *)
+
+Definition proc_to_state {n m} (zx : ZX n m) : ZX 0 (n + m) :=
+  n_cap n ⟷ (n_wire n ↕ zx).
+
+Definition state_to_proc {n m} (zx : ZX 0 (n + m)) : ZX n m :=
+  cast _ _ (eq_sym (Nat.add_0_r _)) 
+    (eq_sym (Nat.add_assoc _ _ _)) 
+    (n_wire n ↕ zx) ⟷ (n_cup n ↕ n_wire m).
+
+Import Setoid. 
+
+Add Parametric Morphism {n m} : (@proc_to_state n m) 
+  with signature proportional_by_1 ==> proportional_by_1 as proc_to_state_mor.
+Proof.
+  unfold proc_to_state.
+  now intros czx czx' ->.
+Qed.
+
+Add Parametric Morphism {n m} : (@state_to_proc n m) 
+  with signature proportional_by_1 ==> proportional_by_1 as state_to_proc_mor.
+Proof.
+  unfold state_to_proc.
+  now intros czx czx' ->.
+Qed.
+
+
+
+Definition state_0 : ZX 0 1 := zx_invsqrt2 ↕ X 0 1 0.
+
+Lemma state_0_defn' : 
+  state_0 = zx_invsqrt2 ↕ X 0 1 0. 
+Proof. reflexivity. Qed.
+
+(* Don't want this to reduce, ever. *)
+Global Opaque state_0.
+
+Definition state_1 : ZX 0 1 := zx_invsqrt2 ↕ X 0 1 PI.
+
+Lemma state_1_defn' : 
+  state_1 = zx_invsqrt2 ↕ X 0 1 PI. 
+Proof. reflexivity. Qed.
+
+(* Don't want this to reduce, ever. *)
+Global Opaque state_1.
+
+Definition state_plus : ZX 0 1 := zx_invsqrt2 ↕ Z 0 1 0.
+
+Lemma state_plus_defn' : 
+  state_plus = zx_invsqrt2 ↕ Z 0 1 0. 
+Proof. reflexivity. Qed.
+  
+(* Don't want this to reduce, ever. *)
+Global Opaque state_plus.
+
+Definition state_minus : ZX 0 1 := zx_invsqrt2 ↕ Z 0 1 PI.
+
+Lemma state_minus_defn' : 
+  state_minus = zx_invsqrt2 ↕ Z 0 1 PI. 
+Proof. reflexivity. Qed.
+
+(* Don't want this to reduce, ever. *)
+Global Opaque state_minus.
+
+
+Definition state_b (b : bool) := if b then state_1 else state_0.
+
+Lemma state_b_defn' b : state_b b = 
+  zx_invsqrt2 ↕ X 0 1 (if b then PI else 0).
+Proof.
+  unfold state_b.
+  rewrite state_0_defn', state_1_defn'.
+  now destruct b.
+Qed.
+
+Fixpoint f_to_state n (f : nat -> bool) : ZX 0 n :=
+  match n with 
+  | 0 => ⦰
+  | S n' => state_b (f O) ↕ f_to_state n' (fun i => f (1 + i)%nat)
+  end.
+
+
+
+Definition uniform_state n : ZX 0 n :=
+  cast _ _ (eq_sym (Nat.mul_0_r _)) (eq_sym (Nat.mul_1_r _))
+    (n_stack n (Z 0 1 0)).
