src/CoreRules/AdditionRules.v
@@ -1,0 +1,193 @@
+Require Import CoreData CapCupRules StackRules 
+  ChoiJamiolchosky GadgetRules ControlizerRules.
+Import Setoid.
+
+
+Lemma zx_plus_defn' {n m} (zx0 zx1 : ZX n m) : 
+  zx0 .+ zx1 ∝= (/√2)^(n+m) .* 
+    state_to_proc (state_1 ⟷ 
+      sum_controlizer (controlizer zx0) (controlizer zx1)).
+Proof.
+  rewrite zx_plus_defn.
+  rewrite gadget_is_scaled_empty, zx_scale_stack_distr_l, stack_empty_l.
+  rewrite const_of_zx_n_stack, const_of_zx_invsqrt2.
+  reflexivity.
+Qed.
+
+Lemma zx_plus_semantics {n m} (zx0 zx1 : ZX n m) : 
+  ⟦ zx0 .+ zx1 ⟧ = 
+  (⟦ zx0 ⟧ .+ ⟦ zx1 ⟧)%M.
+Proof.
+  rewrite zx_plus_defn'.
+  rewrite zx_scale_semantics.
+  unfold state_to_proc.
+  rewrite zx_compose_spec, zx_stack_spec.
+  simpl_cast_semantics.
+  rewrite zx_stack_spec, 2 n_wire_semantics.
+  rewrite sum_controlizer_state_1_semantics by (apply zx_is_controlized).
+  rewrite 2 controlizer_state_1.
+  rewrite 2 zx_scale_semantics.
+  rewrite <- Mscale_plus_distr_r.
+  distribute_scale.
+  restore_dims.
+  unify_pows_two.
+  rewrite Mscale_mult_dist_r, Mscale_assoc.
+  rewrite <- Cpow_mul_l, Cinv_l, Cpow_1_l, Mscale_1_l by nonzero.
+  distribute_plus.
+  restore_dims.
+  unify_pows_two.
+  rewrite Mmult_plus_distr_l.
+  etransitivity. 2:{
+    rewrite <- (proc_to_state_to_proc zx0), <- (proc_to_state_to_proc zx1).
+    unfold state_to_proc.
+    unfold state_to_proc.
+    rewrite 2 zx_compose_spec, zx_stack_spec.
+    simpl_cast_semantics.
+    rewrite 2 zx_stack_spec, 2 n_wire_semantics.
+    reflexivity.
+  }
+  reflexivity.
+Qed.
+
+
+
+Lemma zx_plus_0_l {n m} (zx : ZX n m) : 
+  0 .+ zx ∝= zx.
+Proof.
+  prep_matrix_equivalence.
+  rewrite zx_plus_semantics, zx_zero_semantics, Mplus_0_l.
+  reflexivity.
+Qed.
+
+Lemma zx_plus_0_r {n m} (zx : ZX n m) : 
+  zx .+ 0 ∝= zx.
+Proof.
+  prep_matrix_equivalence.
+  rewrite zx_plus_semantics, zx_zero_semantics, Mplus_0_r.
+  reflexivity.
+Qed.
+
+(* TODO: Other distributivities *)
+
+Lemma zx_plus_comm {n m} (zx0 zx1 : ZX n m) : 
+  zx0 .+ zx1 ∝= zx1 .+ zx0.
+Proof.
+  prep_matrix_equivalence.
+  rewrite 2 zx_plus_semantics, Mplus_comm.
+  reflexivity.
+Qed.
+
+Lemma zx_plus_assoc {n m} (zx0 zx1 zx2 : ZX n m) : 
+  zx0 .+ (zx1 .+ zx2) ∝= zx0 .+ zx1 .+ zx2.
+Proof.
+  prep_matrix_equivalence.
+  rewrite 4 zx_plus_semantics, Mplus_assoc.
+  reflexivity.
+Qed.
+
+(* TODO: Other comm/assoc helpers... *)
+
+
+
+
+Lemma zx_sum_S {n m} (f : nat -> ZX n m) k : 
+  zx_sum f (S k) ∝= zx_sum f k .+ f k.
+Proof.
+  destruct k; [|reflexivity].
+  simpl.
+  now rewrite zx_plus_0_l.
+Qed.
+
+
+
+(* TODO: Other morphism instance (proportionality) *)
+Add Parametric Morphism {n m} : (@zx_sum n m) with signature
+  Morphisms.pointwise_relation nat proportional_by_1 ==> eq ==> proportional_by_1
+  as zx_sum_mor.
+Proof.
+  intros f g Hfg.
+  intros k.
+  induction k; [reflexivity|].
+  now rewrite 2 zx_sum_S, IHk, Hfg.
+Qed.
+
+Lemma zx_sum_semantics {n m} (f : nat -> ZX n m) k : 
+  ⟦ zx_sum f k ⟧ = big_sum (fun i => ⟦ f i ⟧) k.
+Proof.
+  induction k.
+  - apply zx_zero_semantics.
+  - rewrite zx_sum_S.
+    cbn.
+    rewrite zx_plus_semantics, IHk.
+    reflexivity.
+Qed.
+
+Lemma state_of_vector_semantics {n} (v : Vector (2^n)) : WF_Matrix v -> 
+  ⟦ state_of_vector v ⟧ = v.
+Proof.
+  intros Hv.
+  prep_matrix_equivalence.
+  intros i j Hi Hj.
+  replace j with O in * by (simpl in Hj; lia); clear j Hj.
+  unfold state_of_vector.
+  rewrite zx_sum_semantics, Msum_Csum.
+  apply big_sum_unique.
+  exists i.
+  split; [auto|].
+  split.
+  - rewrite zx_scale_semantics, f_to_state_semantics.
+    rewrite <- basis_f_to_vec_alt by auto.
+    rewrite basis_vector_eq_e_i by auto.
+    unfold scale, e_i.
+    bdestructΩ'; lca.
+  - intros j Hj Hji.
+    rewrite zx_scale_semantics, f_to_state_semantics.
+    rewrite <- basis_f_to_vec_alt by auto.
+    rewrite basis_vector_eq_e_i by auto.
+    unfold scale, e_i.
+    bdestructΩ'; lca.
+Qed.
+
+Lemma zx_of_matrix_semantics {n m} (A : Matrix (2^m) (2^n)) : WF_Matrix A -> 
+  ⟦ zx_of_matrix A ⟧ = A.
+Proof.
+  intros HA.
+  prep_matrix_equivalence.
+  unfold zx_of_matrix.
+  (* TODO: Lemma state_to_proc_semantics *)
+  unfold state_to_proc.
+  rewrite zx_compose_spec.
+  simpl_cast_semantics.
+  rewrite (zx_stack_spec _ _ _ _ (n_wire n)).
+  rewrite state_of_vector_semantics by auto_wf.
+  rewrite n_wire_semantics, kron_id_dist_l by auto_wf.
+  restore_dims. 
+  rewrite <- kron_assoc, id_kron by auto_wf.
+  unify_pows_two.
+  rewrite <- Mmult_assoc.
+  rewrite zx_stack_spec, n_wire_semantics.
+  restore_dims.
+  rewrite <- kron_split_diag by auto_wf.
+  rewrite (kron_split_antidiag _ A), kron_1_l by auto_wf.
+  rewrite <- (Mmult_1_r _ _ A) at 2 by auto_wf.
+  unify_pows_two.
+  rewrite Mmult_assoc.
+  (* rewrite Nat.add_0_r. *)
+  apply mmult_mat_equiv_morph; [reflexivity|].
+  generalize (big_yank_r n (Nat.add_assoc _ _ _) eq_refl (Nat.add_0_r _)).
+  unfold proportional_by_1.
+  cbn [Nat.add].
+  simpl_cast_semantics.
+  intros H.
+  rewrite <- n_wire_semantics.
+  etransitivity; [|now rewrite <- H].
+  rewrite zx_compose_spec.
+  simpl_cast_semantics.
+  rewrite zx_stack_spec.
+  restore_dims.
+  pose proof (zx_stack_spec _ _ _ _ (n_cup n) (n_wire n)) as Hrw.
+  cbn [Nat.add] in Hrw.
+  rewrite Hrw.
+  unify_pows_two.
+  reflexivity.
+Qed.
