src/CoreRules/ChoiJamiolchosky.v
@@ -1,0 +1,221 @@
+Require Export CoreData StateRules CoreAutomation GadgetRules StateRules 
+  CastRules StackComposeRules CapCupRules ZXRules.
+
+
+
+Lemma proc_to_state_to_proc {n m} (zx : ZX n m) : 
+  state_to_proc (proc_to_state zx) ∝= zx.
+Proof.
+  unfold state_to_proc, proc_to_state.
+  rewrite n_cap_pullthrough_bot.
+  rewrite stack_nwire_distribute_l.
+  rewrite cast_compose_distribute, compose_assoc.
+  rewrite stack_assoc_back, cast_contract.
+
+  rewrite (cast_compose_l _ _ _ (_ ↕ _)), cast_id. 
+  rewrite <- stack_nwire_distribute_r.
+  rewrite n_cup_pullthrough_bot, transpose_involutive_eq.
+  rewrite stack_nwire_distribute_r.
+  rewrite cast_compose_distribute, stack_assoc, cast_contract.
+  rewrite <- compose_assoc.
+  rewrite cast_compose_eq_mid_join.
+  rewrite <- stack_compose_distr, nwire_removal_l.
+  rewrite push_out_bot, cast_compose_distribute, cast_contract.
+  rewrite compose_assoc, (cast_compose_l _ _ (_ ↕ _)), cast_contract.
+  rewrite n_wire_stack, nwire_removal_r.
+  rewrite big_yank_r.
+  rewrite cast_compose_l.
+  rewrite 2 cast_contract.
+  rewrite 2 cast_id, nwire_removal_r.
+  reflexivity.
+  Unshelve. all: lia.
+Qed.
+
+
+Lemma state_to_proc_to_state {n m} (zx : ZX 0 (n + m)) : 
+  proc_to_state (state_to_proc zx) ∝= zx.
+Proof.
+  unfold state_to_proc, proc_to_state.
+  rewrite stack_nwire_distribute_l.
+  rewrite cast_stack_r, stack_assoc_back, cast_contract.
+  rewrite <- compose_assoc, n_wire_stack.
+  rewrite cast_compose_r, push_out_bot, <- compose_assoc, 
+    cast_compose_eq_mid_join, nwire_removal_r.
+  rewrite <- (push_out_bot zx (n_cap n)).
+  rewrite <- nwire_stack_compose_topleft, cast_compose_distribute, 
+  compose_assoc.
+  rewrite <- n_wire_stack, stack_assoc_back, cast_contract.
+  rewrite cast_id.
+  rewrite (cast_compose_l _ _ (_ ↕ n_wire m)), cast_id.
+  rewrite (stack_assoc_back (n_wire n) (n_cup n) (n_wire m)), cast_contract.
+  rewrite cast_stack_distribute, cast_id.
+  rewrite <- stack_nwire_distribute_r, big_yank_l.
+  rewrite stack_empty_l, n_wire_stack, nwire_removal_r.
+  reflexivity.
+  Unshelve. all: lia.
+Qed.
+
+Lemma zx_scale_proc_to_state {n m} (zx : ZX n m) c : 
+  proc_to_state (c .* zx) ∝= c .* proc_to_state zx.
+Proof.
+  unfold proc_to_state; distribute_zxscale.
+  reflexivity.
+Qed.
+
+Lemma zx_scale_state_to_proc {n m} (zx : ZX 0 (n + m)) c : 
+  state_to_proc (c .* zx) ∝= c .* state_to_proc zx.
+Proof.
+  unfold state_to_proc.
+  rewrite zx_scale_stack_distr_r, zx_scale_cast.
+  distribute_zxscale.
+  reflexivity.
+Qed.
+
+#[export] Hint Rewrite 
+  @zx_scale_proc_to_state @zx_scale_state_to_proc : zxscale_db.
+
+Lemma colorswap_proc_to_state {n m} (zx : ZX n m) : 
+  ⊙ (proc_to_state zx) ∝= proc_to_state (⊙ zx).
+Proof.
+  unfold proc_to_state; cbn [color_swap]; 
+  autorewrite with colorswap_db.
+  reflexivity.
+Qed.
+
+Lemma colorswap_state_to_proc {n m} (zx : ZX 0 (n + m)) : 
+  ⊙ (state_to_proc zx) ∝= state_to_proc (⊙ zx).
+Proof.
+  unfold state_to_proc; cbn [color_swap]; 
+  autorewrite with colorswap_db.
+  cbn [color_swap].
+  autorewrite with colorswap_db.
+  reflexivity.
+Qed.
+
+#[export] Hint Rewrite 
+  @colorswap_proc_to_state @colorswap_state_to_proc : colorswap_db.
+
+
+Lemma proc_to_state_Z n m α : proc_to_state (Z n m α) ∝=
+  Z 0 (n + m) α.
+Proof.
+  unfold proc_to_state.
+  now rewrite <- Z_n_wrap_over_l_base.
+Qed.
+
+Lemma state_to_proc_Z n m α : state_to_proc (Z 0 (n + m) α) ∝=
+  Z n m α.
+Proof.
+  now rewrite <- proc_to_state_Z, proc_to_state_to_proc.
+Qed.
+
+Local Opaque proc_to_state state_to_proc.
+Lemma proc_to_state_X n m α : proc_to_state (X n m α) ∝=
+  X 0 (n + m) α.
+Proof. colorswap_of (proc_to_state_Z n m α). Qed.
+Lemma state_to_proc_X n m α : state_to_proc (X 0 (n + m) α) ∝=
+  X n m α.
+Proof. colorswap_of (state_to_proc_Z n m α). Qed.
+Local Transparent proc_to_state state_to_proc.
+
+
+Lemma proc_to_state_state {n} (zx : ZX 0 n) : 
+  proc_to_state zx ∝= zx.
+Proof.
+  unfold proc_to_state.
+  rewrite n_cap_0_empty.
+  cleanup_zx.
+  reflexivity.
+Qed.
+
+
+Lemma state_to_proc_diagrams {n m} (zx zx' : ZX 0 (n + m)) : 
+  state_to_proc zx ∝= state_to_proc zx' ->
+  zx ∝= zx'.
+Proof.
+  intros H%proc_to_state_mor.
+  now rewrite 2 state_to_proc_to_state in H.
+Qed.
+
+Lemma proc_to_state_diagrams {n m} (zx zx' : ZX n m) : 
+  proc_to_state zx ∝= proc_to_state zx' ->
+  zx ∝= zx'.
+Proof.
+  intros H%state_to_proc_mor.
+  now rewrite 2 proc_to_state_to_proc in H.
+Qed.
+
+Lemma state_to_proc_diagrams_iff {n m} (zx zx' : ZX 0 (n + m)) : 
+  state_to_proc zx ∝= state_to_proc zx' <->
+  zx ∝= zx'.
+Proof.
+  split; [apply state_to_proc_diagrams | now intros ->].
+Qed.
+
+Lemma proc_to_state_diagrams_iff {n m} (zx zx' : ZX n m) : 
+  proc_to_state zx ∝= proc_to_state zx' <->
+  zx ∝= zx'.
+Proof.
+  split; [apply proc_to_state_diagrams | now intros ->].
+Qed.
+
+Lemma state_to_proc_eq_l {n m} (zx : ZX 0 (n + m)) zx' : 
+  state_to_proc zx ∝= zx' <-> zx ∝= proc_to_state zx'.
+Proof.
+  rewrite <- (proc_to_state_to_proc zx') at 1.
+  apply state_to_proc_diagrams_iff.
+Qed.
+
+Lemma state_to_proc_eq_r {n m} zx (zx' : ZX 0 (n + m)) : 
+  zx ∝= state_to_proc zx' <-> proc_to_state zx ∝= zx'.
+Proof.
+  rewrite <- (proc_to_state_to_proc zx) at 1.
+  apply state_to_proc_diagrams_iff.
+Qed.
+
+Lemma proc_to_state_eq_l {n m} zx (zx' : ZX 0 (n + m)) : 
+  proc_to_state zx ∝= zx' <-> zx ∝= state_to_proc zx'.
+Proof.
+  rewrite <- (state_to_proc_to_state zx') at 1.
+  apply proc_to_state_diagrams_iff.
+Qed.
+
+Lemma proc_to_state_eq_r {n m} (zx : ZX 0 (n + m)) zx' : 
+  zx ∝= proc_to_state zx' <-> state_to_proc zx ∝= zx'.
+Proof.
+  rewrite <- (state_to_proc_to_state zx) at 1.
+  apply proc_to_state_diagrams_iff.
+Qed.
+
+Lemma proc_to_state_n_wire n : proc_to_state (n_wire n) ∝= n_cap n.
+Proof.
+  unfold proc_to_state.
+  rewrite n_wire_stack, nwire_removal_r.
+  reflexivity.
+Qed.
+
+Lemma state_to_proc_n_cap n : state_to_proc (n_cap n) ∝= n_wire n.
+Proof.
+  rewrite state_to_proc_eq_l, proc_to_state_n_wire.
+  reflexivity.
+Qed.
+
+Lemma proc_to_state_alt {n m} (zx : ZX n m) : 
+  proc_to_state zx ∝= n_cap m ⟷ ((zx ⊤) ↕ n_wire m).
+Proof.
+  unfold proc_to_state.
+  apply n_cap_pullthrough_bot.
+Qed.
+
+Lemma proc_to_state_effect {n} (zx : ZX n 0) : 
+  proc_to_state zx ∝= zx⊤ ↕ ⦰.
+Proof.
+  unfold proc_to_state.
+  rewrite n_cap_pullthrough_bot, n_cap_0_empty, compose_empty_l.
+  reflexivity.
+Qed.
+
+Lemma state_to_proc_n_cup n : proc_to_state (n_cup n) ∝= n_cap n ↕ ⦰.
+Proof.
+  apply proc_to_state_effect.
+Qed.
