src/CoreRules/CoreRules.v
@@ -7,3 +7,9 @@ Require Export CoreAutomation.
 Require Export XRules.
 Require Export ZXRules.
 Require Export SwapRules.
+Require Export GadgetRules.
+Require Export StateRules.
+Require Export ChoiJamiolchosky.
+Require Export ControlizerRules.
+Require Export AdditionRules.
+
