src/CoreRules/StateRules.v
@@ -1,0 +1,382 @@
+Require Import CoreData GadgetRules CoreAutomation StackComposeRules.
+
+Open Scope ZX_scope.
+
+Lemma state_0_defn : 
+  state_0 ∝= /√2 .* X 0 1 0. 
+Proof.
+  rewrite state_0_defn'.
+  rewrite gadget_is_scaled_empty; distribute_zxscale.
+  rewrite stack_empty_l, const_of_zx_invsqrt2. 
+  reflexivity.
+Qed.
+
+Lemma state_0_semantics : ⟦ state_0 ⟧ = ∣0⟩.
+Proof.
+  prep_matrix_equivalence.
+  rewrite state_0_defn.
+  rewrite zx_scale_semantics.
+  compute_matrix (⟦ X 0 1 0 ⟧).
+  rewrite kron_1_l by auto_wf.
+  rewrite Cexp_0; Csimpl.
+  unfold hadamard; simpl.
+  rewrite make_WF_equiv.
+  by_cell; autounfold with U_db; unfold list2D_to_matrix; simpl;
+  [C_field; lca | lca].
+Qed.
+
+
+Lemma state_1_defn : 
+  state_1 ∝= /√2 .* X 0 1 PI. 
+Proof.
+  rewrite state_1_defn'.
+  rewrite gadget_is_scaled_empty; distribute_zxscale.
+  rewrite stack_empty_l, const_of_zx_invsqrt2. 
+  reflexivity.
+Qed.
+
+Lemma state_1_semantics : ⟦ state_1 ⟧ = ∣1⟩.
+Proof.
+  prep_matrix_equivalence.
+  rewrite state_1_defn.
+  rewrite zx_scale_semantics.
+  compute_matrix (⟦ X 0 1 PI ⟧).
+  rewrite kron_1_l by auto_wf.
+  rewrite Cexp_PI.
+  unfold hadamard; simpl.
+  rewrite make_WF_equiv.
+  by_cell; autounfold with U_db; unfold list2D_to_matrix; simpl;
+  [lca | C_field; lca].
+Qed.
+
+Lemma state_plus_defn : 
+  state_plus ∝= /√2 .* Z 0 1 0. 
+Proof.
+  rewrite state_plus_defn'.
+  rewrite gadget_is_scaled_empty; distribute_zxscale.
+  rewrite stack_empty_l, const_of_zx_invsqrt2. 
+  reflexivity.
+Qed.
+
+Lemma state_plus_semantics : ⟦ state_plus ⟧ = ∣+⟩.
+Proof.
+  prep_matrix_equivalence.
+  rewrite state_plus_defn.
+  rewrite zx_scale_semantics.
+  compute_matrix (⟦ Z 0 1 0 ⟧).
+  rewrite Cexp_0.
+  rewrite make_WF_equiv.
+  unfold xbasis_plus;
+  by_cell; autounfold with U_db; unfold list2D_to_matrix; simpl; lca.
+Qed.
+
+Lemma state_minus_defn : 
+  state_minus ∝= /√2 .* Z 0 1 PI. 
+Proof. 
+  rewrite state_minus_defn'.
+  rewrite gadget_is_scaled_empty; distribute_zxscale.
+  rewrite stack_empty_l, const_of_zx_invsqrt2. 
+  reflexivity.
+Qed.
+
+Lemma state_minus_semantics : ⟦ state_minus ⟧ = ∣-⟩.
+Proof.
+  prep_matrix_equivalence.
+  rewrite state_minus_defn.
+  rewrite zx_scale_semantics.
+  compute_matrix (⟦ Z 0 1 PI ⟧).
+  rewrite Cexp_PI.
+  rewrite make_WF_equiv.
+  unfold xbasis_minus;
+  by_cell; autounfold with U_db; unfold list2D_to_matrix; simpl; lca.
+Qed.
+
+
+Lemma state_0_colorswap : ⊙ state_0 ∝= state_plus.
+Proof.
+  rewrite state_0_defn, state_plus_defn.
+  rewrite zx_scale_colorswap.
+  reflexivity.
+Qed.
+
+Lemma state_1_colorswap : ⊙ state_1 ∝= state_minus.
+Proof.
+  rewrite state_1_defn, state_minus_defn.
+  rewrite zx_scale_colorswap.
+  reflexivity.
+Qed.
+
+Lemma state_plus_colorswap : ⊙ state_plus ∝= state_0.
+Proof.
+  apply colorswap_diagrams_eq.
+  rewrite colorswap_involutive.
+  now rewrite state_0_colorswap.
+Qed.
+
+Lemma state_minus_colorswap : ⊙ state_minus ∝= state_1.
+Proof.
+  apply colorswap_diagrams_eq.
+  rewrite colorswap_involutive.
+  now rewrite state_1_colorswap.
+Qed.
+
+#[export] Hint Rewrite state_0_colorswap state_1_colorswap
+  state_plus_colorswap state_minus_colorswap : colorswap_db.
+
+
+
+
+Lemma semantics_compose_state_0_l {n} (zx : ZX 1 n) : 
+  ⟦ state_0 ⟷ zx ⟧ = get_col (⟦ zx ⟧) 0.
+Proof.
+  simpl.
+  rewrite state_0_semantics.
+  rewrite qubit0_to_ei.
+  now rewrite matrix_by_basis by lia.
+Qed.
+
+Lemma semantics_compose_state_1_l {n} (zx : ZX 1 n) : 
+  ⟦ state_1 ⟷ zx ⟧ = get_col (⟦ zx ⟧) 1.
+Proof.
+  simpl.
+  rewrite state_1_semantics.
+  rewrite qubit1_to_ei.
+  now rewrite matrix_by_basis by lia.
+Qed.
+
+
+
+Lemma semantics_by_states_1_n {n} (zx : ZX 1 n) : 
+  ⟦ zx ⟧ = smash (⟦ state_0 ⟷ zx ⟧) (⟦ state_1 ⟷ zx ⟧).
+Proof.
+  prep_matrix_equivalence.
+  rewrite semantics_compose_state_0_l, semantics_compose_state_1_l.
+  intros i j Hi Hj.
+  unfold smash, get_col.
+  simpl in *.
+  destruct j; [|replace j with O in * by lia];
+  Modulus.bdestructΩ'.
+Qed.
+
+Lemma prop_eq_by_eq_on_states_1_n {n} (zx zx' : ZX 1 n) : 
+  state_0 ⟷ zx ∝= state_0 ⟷ zx' ->
+  state_1 ⟷ zx ∝= state_1 ⟷ zx' ->
+  zx ∝= zx'.
+Proof.
+  intros H0 H1.
+  prep_matrix_equivalence.
+  rewrite 2 semantics_by_states_1_n.
+  rewrite H0, H1.
+  reflexivity.
+Qed.
+
+Lemma prop_eq_by_eq_on_states_step {n m} (zx zx' : ZX (S n) m) : 
+  state_0 ↕ n_wire n ⟷ zx ∝= state_0 ↕ n_wire n ⟷ zx' ->
+  state_1 ↕ n_wire n ⟷ zx ∝= state_1 ↕ n_wire n ⟷ zx' ->
+  zx ∝= zx'.
+Proof.
+  intros H0 H1.
+  prep_matrix_equivalence.
+  intros i j Hi Hj.
+  bdestruct (j <? 2 ^ n).
+  - generalize (equal_f (equal_f H0 i) j).
+    rewrite 2 zx_compose_spec, zx_stack_spec.
+    rewrite state_0_semantics, n_wire_semantics.
+    rewrite qubit0_to_ei.
+    replace (2 ^ (1 + n))%nat with (2 * (2 ^ n))%nat by (simpl; lia).
+    rewrite (Nat.pow_add_r 2 0 n), (Nat.pow_0_r).
+    rewrite 2 Mmult_kron_e_i_I_r by solve [restore_dims; auto_wf | lia].
+    rewrite 2 make_WF_equiv by lia.
+    rewrite Nat.mul_0_r, Nat.add_0_l.
+    easy.
+  - generalize (equal_f (equal_f H1 i) (j - 2 ^ n)%nat).
+    rewrite 2 zx_compose_spec, zx_stack_spec.
+    rewrite state_1_semantics, n_wire_semantics.
+    rewrite qubit1_to_ei.
+    replace (2 ^ (1 + n))%nat with (2 * (2 ^ n))%nat by (simpl; lia).
+    rewrite (Nat.pow_add_r 2 0 n), (Nat.pow_0_r).
+    rewrite 2 Mmult_kron_e_i_I_r by solve [restore_dims; auto_wf | lia].
+    rewrite 2 make_WF_equiv by (simpl in Hj; lia).
+    rewrite Nat.mul_1_r.
+    rewrite (Nat.add_comm (2^n) (j - _)), Nat.sub_add by lia.
+    easy.
+Qed.
+
+
+
+Lemma prop_eq_by_eq_on_state_b_1_n {n} (zx zx' : ZX 1 n) : 
+  (forall b, state_b b ⟷ zx ∝= state_b b ⟷ zx') ->
+  zx ∝= zx'.
+Proof.
+  intros Hb.
+  apply prop_eq_by_eq_on_states_1_n.
+  - apply (Hb false).
+  - apply (Hb true).
+Qed.
+
+
+
+
+
+
+
+
+
+
+
+
+
+
+
+
+Lemma state_b_semantics b : 
+  ⟦ state_b b ⟧ = ket (Nat.b2n b).
+Proof.
+  destruct b.
+  - apply state_1_semantics.
+  - apply state_0_semantics.
+Qed.
+
+Lemma f_to_state_semantics n f : 
+  ⟦ f_to_state n f ⟧ = f_to_vec n f.
+Proof.
+  revert f;
+  induction n; intros f.
+  - reflexivity. 
+  - cbn [f_to_state].
+    rewrite (@zx_stack_spec 0 1 0 n).
+    rewrite state_b_semantics.
+    rewrite (f_to_vec_split'_eq 1 n).
+    rewrite IHn.
+    f_equal.
+    simpl.
+    now rewrite kron_1_l by auto_wf.
+Qed.
+
+Lemma f_to_state_split n m f : 
+  f_to_state (n + m) f ∝= f_to_state n f ↕ f_to_state m (fun i => f (n + i)%nat).
+Proof.
+  prep_matrix_equivalence.
+  cbn.
+  rewrite 3 f_to_state_semantics.
+  now rewrite f_to_vec_split'_eq.
+Qed.
+
+Lemma f_to_state_merge n m f g : 
+  f_to_state m f ↕ f_to_state n g ∝=
+  f_to_state (m + n) (fun x => if x <? m then f x else g (x - m)%nat).
+Proof.
+  prep_matrix_equivalence.
+  cbn.
+  rewrite 3 f_to_state_semantics.
+  now rewrite f_to_vec_merge.
+Qed.
+
+
+(* Rules about the zero element zx_zero *)
+
+
+Lemma zx_zero_semantics n m : ⟦@zx_zero n m⟧ = Zero.
+Proof.
+  rewrite zx_zero_defn.
+  rewrite zx_scale_semantics.
+  apply Mscale_0_l.
+Qed.
+
+Lemma zx_scale_0_l {n m} (zx : ZX n m) : 
+  C0 .* zx ∝= 0.
+Proof.
+  prep_matrix_equivalence.
+  rewrite zx_scale_semantics, zx_zero_semantics.
+  now rewrite Mscale_0_l.
+Qed.
+
+Lemma zx_scale_0_r {n m} c : 
+  c .* (@zx_zero n m) ∝= 0.
+Proof.
+  rewrite zx_zero_defn.
+  distribute_zxscale.
+  now rewrite Cmult_0_r.
+Qed.
+
+Lemma stack_0_l {n0 m0 n1 m1} (zx : ZX n1 m1) : 
+  (@zx_zero n0 m0) ↕ zx ∝= 0.
+Proof.
+  rewrite zx_zero_defn.
+  distribute_zxscale.
+  now rewrite zx_scale_0_l.
+Qed.
+
+Lemma stack_0_r {n0 m0 n1 m1} (zx : ZX n0 m0) : 
+  zx ↕ (@zx_zero n1 m1) ∝= 0.
+Proof.
+  rewrite zx_zero_defn.
+  distribute_zxscale.
+  now rewrite zx_scale_0_l.
+Qed.
+
+Lemma compose_0_l {n m o} (zx : ZX m o) : 
+  (@zx_zero n m) ⟷ zx ∝= 0.
+Proof.
+  rewrite zx_zero_defn.
+  distribute_zxscale.
+  now rewrite zx_scale_0_l.
+Qed.
+
+Lemma compose_0_r {n m o} (zx : ZX n m) : 
+  zx ⟷ (@zx_zero m o) ∝= 0.
+Proof.
+  rewrite zx_zero_defn.
+  distribute_zxscale.
+  now rewrite zx_scale_0_l.
+Qed.
+
+Lemma cast_0 n m {n' m'} prfn prfm : 
+  cast n m prfn prfm (@zx_zero n' m') = 0.
+Proof.
+  now subst.
+Qed.
+
+Lemma n_stack_zx_zero k n m : k <> O ->
+  k ⇑ (@zx_zero n m) ∝= 0.
+Proof.
+  intros H.
+  destruct k; [easy|].
+  simpl.
+  now rewrite stack_0_l.
+Qed.
+
+(* Lemma n_compose_zx_zero k n : k <> O -> 
+  n_compose k (@zx_zero n n) ∝= zx_zero.
+Proof.
+  intros Hk.
+  destruct k; [easy|].
+  simpl.
+  now rewrite compose_0_l.
+Qed. *)
+
+Lemma zx_zero_transpose n m : (@zx_zero n m) ⊤ ∝= 0.
+Proof.
+  rewrite zx_zero_defn.
+  distribute_zxscale.
+  now rewrite zx_scale_0_l.
+Qed.
+
+Lemma zx_zero_adjoint n m : (@zx_zero n m) † ∝= 0.
+Proof.
+  rewrite zx_zero_defn.
+  distribute_zxscale.
+  now rewrite Cconj_R, zx_scale_0_l.
+Qed.
+
+Lemma zx_zero_colorswap n m : ⊙ (@zx_zero n m) ∝= 0.
+Proof.
+  rewrite zx_zero_defn.
+  distribute_zxscale.
+  now rewrite zx_scale_0_l.
+Qed.
+
+#[export] Hint Rewrite zx_zero_transpose : transpose_db.
+#[export] Hint Rewrite zx_zero_adjoint : adjoint_db.
+#[export] Hint Rewrite zx_zero_colorswap : colorswap_db.
+
