src/CoreRules/SwapRules.v
@@ -78,7 +78,7 @@ Proof.
 Qed.
 
 Lemma swap_spec' : swap = ((ket 0 × bra 0)  ⊗ (ket 0 × bra 0) .+ (ket 0 × bra 1)  ⊗ (ket 1 × bra 0)
-  .+ (ket 1 × bra 0)  ⊗ (ket 0 × bra 1) .+ (ket 1 × bra 1)  ⊗ (ket 1 × bra 1)).
+  .+ (ket 1 × bra 0)  ⊗ (ket 0 × bra 1) .+ (ket 1 × bra 1)  ⊗ (ket 1 × bra 1))%M.
 Proof.
   prep_matrix_equivalence.
   by_cell; lazy; lca.
